Stopping here.

src/asynchronous_automata.lean
@@ -279,17 +279,14 @@ notation `#[` arr:(foldr `,` (h t, array.push_back t h) array.nil `]`) := arr.re
 def array.to_vector {n α} (arr : array n α) : vector α n := 
   ⟨arr.to_list, array.to_list_length arr⟩ 
 
-infix `⇨`:40 := rbmap
-
-def ACA_rules.from_list : list (array 2 (array 8 (fin 2))) → template bool ⇨ template bool
+def ACA_rules.from_list : list (array 2 (array 8 (fin 2))) → template bool ~> template bool
   | l :=
-    let to_templates : array 2 (array 8 (fin 2)) → (template bool × template bool) :=
+    let to_templates : array 2 (array 8 (fin 2)) → (Σ _, template bool) :=
       λ arr, 
         match (arr.map array.to_template).to_vector with
         | ⟨[old, new], _⟩ := ⟨old, new⟩
         end
-      in
-    rbmap_of (l.map to_templates)
+      in (l.map to_templates).to_finmap
 
 def convert_from_dixons : array 8 (fin 2) → array 8 (fin 2)
   | arr := 
@@ -311,7 +308,7 @@ def LHZ_list :=
 		#[#[0,0,1,1,0,1,1,1], #[1,1,0,1,1,1,0,0]]  -- Toggle Memory
   ]
 
-def LHZ_base : template bool ⇨ template bool :=
+def LHZ_base : template bool ~> template bool :=
   ACA_rules.from_list LHZ_list
 
 def template.print {α} (to_char : α → char) (t : template α) : string := 
@@ -407,6 +404,9 @@ end symmetries
 def finset.as_list {α β : Type} (f : list α → β) (p : _) : finset α → β
   | ⟨ms, ms_no_dup⟩ := quotient.lift f p ms
 
+def finmap.as_list {α : Type} {β : α → Type} {γ : Type} (f : list (sigma β) → γ) (p : _) : finmap β → γ
+  | ⟨ms, nodup⟩ := quotient.lift f p ms
+
 def on_equiv {α β} (π : α ≃ β) (f : β → β) (a : α) : α := π.symm (f (π a))
 
 lemma on_equiv.id {α β} (π : α ≃ β) (a : α) :
@@ -440,7 +440,7 @@ lemma template.precompose_functorial {α} (t : template α) (f g : vonNeumann �
     rw on_equiv.functorial,
   }
 
-def on_rule {α} (π : ¡vonNeumann) : ¡(template α × template α) :=
+def on_rule {α} (π : ¡vonNeumann) : ¡(Σ _:template α, template α) :=
   { 
     to_fun := λ rule, ⟨rule.1.precompose π, rule.2.precompose π⟩,
     inv_fun := λ rule, ⟨rule.1.precompose π.symm, rule.2.precompose π.symm⟩,
@@ -455,6 +455,7 @@ def on_rule {α} (π : ¡vonNeumann) : ¡(template α × template α) :=
       have : (λ (x : vonNeumann), x) = id := by {funext, simp},
       simp_rw this,
       simp_rw template.precompose_id,
+      split; refl,
     },
     right_inv := 
     by {
@@ -467,78 +468,64 @@ def on_rule {α} (π : ¡vonNeumann) : ¡(template α × template α) :=
       have : (λ (x : vonNeumann), x) = id := by {funext, simp},
       simp_rw this,
       simp_rw template.precompose_id,
+      split; refl,
     }
   }
 
-def to_rbmap (α) [linear_order α] (base : list (template α × template α)) (πs : list ¡vonNeumann) := 
-  rbmap_of $ has_seq.seq (πs.map (equiv.to_fun ∘ on_rule)) base
+def alist.elaborate {α} [linear_order α] (πs : finset ¡vonNeumann) (base : alist (λ_ : template α, template α))  : 
+  alist (λ_ : template α, template α) :=
+    (has_seq.seq (πs.map (equiv.to_fun ∘ on_rule)) base.to_finset).to_alist
 
-def prod_to_sigma {α β} (p : α × β) : (Σ _ : α, β) := ⟨p.1, p.2⟩
+def rules.elaborate {α} [linear_order α]
+  (base : template α ~> template α) (sym : symmetries) : template α ~> template α :=
+   base.lift_on (alist.elaborate sym.to_finset)
 
-axiom rbmap.ext {α β} [linear_order α] (x y : α ⇨ β) : (∀ a : α, x.find a = y.find a) → x = y
+def LHZ := rules.elaborate LHZ_base symmetries.rotate4
 
-lemma list.cons_cons_eq_append {α} (x y : α) (l : list α) : x :: y :: l = [x, y] ++ l := 
-  by {
-    symmetry,
-    rw list.append_eq_cons_iff,
-    right,
-    use [[y]],
-    split, refl,
-    symmetry,
-    rw list.append_eq_cons_iff,
-    right,
-    use list.nil,
-    split, refl,
-    rw list.nil_append,
+inductive step {α} [linear_order α] (rules : template α ~> template α) {n m : ℕ} : 
+  ACA_board (n+1) (m+1) α → ACA_board (n+1) (m+1) α → Prop
+  | intro : ∀ (p : fin (n+1) × fin (m+1)) (mat : ACA_board (n+1) (m+1) α) {b},
+    b ∈ rules.find (read_template mat p) → step mat (write_template mat p b)
+
+instance {α} [fintype α] : fintype (xcell α) :=
+  {
+    elems := finset.map ⟨xcell.mk, by {intros a₁ a₂ h, injection h}⟩ (fintype.elems _),
+    complete := by {
+      intros x,
+      cases x,
+      rw finset.mem_map,
+      simp_rw exists_prop,
+      simp_rw function.embedding.coe_fn_mk,
+      rw exists_eq_right,
+      apply fintype.complete,
+    }
   }
 
-lemma list.sorted_perm_eq {α : Type} [partial_order α] (l₁ l₂ : list α) : 
-  l₁.sorted (≤) → l₂.sorted (≤) → l₁ ~ l₂ → l₁ = l₂ :=
-by {
-  intros s₁ s₂ p,
-  induction p,
-  case nil {refl},
-  case cons {
-    congr,
-    apply p_ih (list.sorted_of_sorted_cons s₁) (list.sorted_of_sorted_cons s₂),
-  },
-  case swap {
-    suffices : p_x = p_y,
-      {congr, exact this.symm, exact this},
-    apply has_le.le.antisymm,
-    cases s₂ with _ _ s_x s₂,
-    apply s_x, left, refl,
-    cases s₁ with _ _ s_y s₁,
-    apply s_y, left, refl,
-    
+instance {α} [fintype α] (n m) : fintype (ACA_board n m α) := 
+{ 
+  elems := finset.map ⟨aMatrix.mk, by {intros a₁ a₂ h, injection h}⟩ (fintype.elems _),
+  complete := by {
+    intros x,
+    cases x,
+    rw finset.mem_map,
+    simp_rw exists_prop,
+    simp_rw function.embedding.coe_fn_mk,
+    use x,
+    split,
+    apply fintype.complete,
+    refl
   }
 }
 
-lemma list.merge_sort.merge_of_parts {α : Type} [linear_order α] (l₁ l₂ : list α) :
-  let ms := list.merge_sort ((≤) : α → α → Prop) in
-   ms (l₁ ++ l₂) = list.merge (≤) (ms l₁) (ms l₂) :=
-by {
-  simp,
+def is_head {n m} (mat : ACA_board (n+1) (m+1) bool) (pos : fin (n+1) × fin (m+1)) : Prop :=
+  read_template mat pos ∈ LHZ
 
-}
+instance {n m} (mat : ACA_board (n+1) (m+1) bool) (pos : fin (n+1) × fin (m+1)) : decidable (is_head mat pos) :=
+  if H : LHZ.contains (read_template mat pos)
+    then is_false sorry
+    else is_true sorry
 
-def finset.to_sorted_list {α : Type} [linear_order α] (s : finset α) : list α :=
-  s.as_list (list.merge_sort has_le.le) 
-    (by {
-      intros a b p,
-      unfold_projs at p,
-      induction p,
-      case nil {refl},
-      case cons {
-        simp_rw list.merge_sort_eq_insertion_sort at *,
-        simp_rw list.insertion_sort_cons_eq_take_drop,
-        congr; exact p_ih,
-      },
-      {
-        simp_rw list.cons_cons_eq_append,
-      },
-    })
+theorem LHZ_preserves_heads (n m : ℕ) (m₁ m₂ : ACA_board (n+1) (m+1) bool) (h : step LHZ m₁ m₂) :
+  fintype.card {p // is_head m₁ p} = fintype.card {p // is_head m₂ p} := {
 
--- def rules.elaborate {α} [linear_order α]
---   (base : template α ⇨ template α) (sym : symmetries) : template α ⇨ template α :=
---   sym.to_finset.to_sorted_list
+  }
